sol04

Program-proofs/Exercises/2D-counting/prob04/sol04.dfy
@@ -1,7 +1,53 @@
-/* file: sol02.dfy
+/* file: sol04.dfy
    author: David De Potter
    description: extra practice in Dafny, 2D counting, 
-   solution to prob02
-   This is exercise 9.3 from the PC reader
+   solution to prob04
+   This is exercise 9.5 from the PC reader
 */
+
+ghost predicate IncrIncr(f:(int,int) -> int) 
+{
+  (forall i,j,k:: i < j  ==>  f(i,k) < f(j,k)) &&
+  (forall i,j,k:: j < k  ==>  f(i,j) < f(i,k))
+}
+
+function ord(b:bool): int
+{
+  if b then 1 else 0
+}
+
+ghost function F(g:(int,int) -> int, x:nat, y:nat, m:nat): int
+requires IncrIncr(g)
+decreases (m - x) + y
+{   
+  if x >= m || y <= 0 then 0
+  else if g(x, y - 1) < y - 1 then F(g, x + 1, y, m)
+  else F(g, x, y - 1, m) + ord(g(x, y - 1) == y - 1)
+}
+
+method problem04(g:(int,int) -> int, m:nat, n:nat) 
+returns (r: int)
+requires IncrIncr(g)
+ensures r == F(g, 0, n, m)
+{
+  var x, y, z := 0, n, 0;
+
+  while x < m && y > 0
+  invariant z + F(g,x,y,m) == F(g,0,n,m)
+  decreases (m - x) + y
+  {   
+    if g(x, y - 1) < y - 1
+    {   
+      x := x + 1;
+    }
+
+    else
+    { 
+      z := z + ord(g(x, y - 1) == y - 1);
+      y := y - 1;
+    }
+  }
+    
+  r := z;
+}
 
